bin/rust/rocq/Values.v
@@ -1,0 +1,43 @@
+From Coq Require Export QArith.
+
+Parameter Ptr: Set.
+
+Parameter null_ptr: Ptr.
+
+Inductive Value :=
+| VPtr(ptr: Ptr)
+| VBool(b: bool)
+| VReal(q: Q)
+| VDummy (* Used as the value of nonsensical expressions *)
+| VSome(v: Value)
+| VTuple0
+.
+
+Definition value_eqb(v1 v2: Value): bool.
+Admitted.
+
+Lemma value_eqb_def_(v1 v2: Value): (VBool (value_eqb v1 v2) = VBool true) = (v1 = v2).
+Admitted.
+
+From Coq Require Export List String.
+Import ListNotations.
+
+Fixpoint assoc{T}(x: string)(xys: list (string * T)): option T :=
+  match xys with
+    [] => None
+  | (x', y)::xys =>
+    if string_dec x x' then
+      Some y
+    else
+      assoc x xys
+  end.
+
+Fixpoint combine_{A B}(xs: list A)(ys: list B): list (A * B) * (list A * list B) :=
+  match xs, ys with
+    [], ys => ([], ([], ys))
+  | xs, [] => ([], (xs, []))
+  | (x::xs), (y::ys) =>
+    let '(xys, (xs, ys)) := combine_ xs ys in
+    ((x, y)::xys, (xs, ys))
+  end.
+
